Veir/Rewriter/WellFormed/Builder/BlockOperands.lean
@@ -110,14 +110,8 @@ theorem Rewriter.pushBlockOperand_WellFormed (hOpWf : ctx.WellFormed) :
     all_goals grind [Rewriter.pushBlockOperand, Operation.WellFormed, OperationPtr.getBlockOperand]
   case blocks =>
     intros bl hbl
-    constructor
-    · grind
-    · intros i hi
-      have ⟨h₁, h₂, h₃⟩ := hOpWf.blocks bl (by grind)
-      grind
-    · intros i hi
-      have ⟨h₁, h₂, h₃⟩ := hOpWf.blocks bl (by grind)
-      grind
+    have ⟨h₁, h₂, h₃, h₄, h₅⟩ := hOpWf.blocks bl (by grind)
+    constructor <;> grind
   case regions =>
     intros reg hreg
     have ⟨h₁, h₂⟩ := hOpWf.regions reg (by grind)
